\begin{figure}
{\small \[
\begin{array}{rcl|rcl|rcl}
{(\Gamma)^\circ} & & &
{(\Delta)^\circ} & & &
{(\Gamma)^\bullet} & & 
\\
(\cdot)^\circ & \!\!\!=\!\!\! & \cdot &
(\cdot)^\circ & \!\!\!=\!\!\! & \cdot &
(\cdot)^\bullet & \!\!\!=\!\!\! & \cdot 
\\
(\Gamma, A^-)^\circ & \!\!\!=\!\!\! & (\Gamma)^\circ, (A^-)^\circ &
(\Delta, A^+)^\circ & \!\!\!=\!\!\! & (\Delta)^\circ, (A^+)^\circ &
(\Gamma, A)^\bullet & \!\!\!=\!\!\! & (\Gamma)^\bullet, (A)^\ominus 
\\
& & & 
(\Delta, A^-)^\circ & \!\!\!=\!\!\! & (\Delta)^\circ, (A^-)^\circ &
& & 
\\
(U)^\circ & & &
(\Delta, [ A^- ])^\circ & \!\!\!=\!\!\! & (\Delta)^\circ, (A^-)^\circ & 
(\Delta)^\bullet & &
\\
(A^-)^\circ &  \!\!\!=\!\!\! & (A^-)^\circ &
(\Delta, \langle p^+ \rangle)^\circ & \!\!\!=\!\!\! & (\Delta)^\circ, p^+ & 
(\Delta, p^+)^\bullet & \!\!\!=\!\!\! & (\Delta)^\bullet, \langle p^+ \rangle
\\
(A^+)^\circ &  \!\!\!=\!\!\! & (A^+)^\circ &
& & &
(\Delta, A)^\bullet & \!\!\!=\!\!\! & (\Delta)^\bullet, A^\ominus ~~(A \neq p^+)
\\
([A^+])^\circ &  \!\!\!=\!\!\! & (A^+)^\circ &
& & &
& &
\\
(\langle p^- \rangle)^\circ &  \!\!\!=\!\!\! & p^- &
& & & 
(C)^\bullet & &
\\
& & & 
& & &
(p^-)^\bullet & \!\!\!=\!\!\! & \langle p^- \rangle
\\
& & & 
& & &
(A)^\bullet & \!\!\!=\!\!\! & A^\oplus ~~(A \neq p^+)
\end{array}\]}
\caption{Lifting erasure and polarization (Figure~\ref{fig:lin-shift}) to
contexts and succeedents.}
\label{fig:lin-shift-ctx}
\end{figure}
